LambdaS5/coq/LjsStore.v
@@ -2,17 +2,23 @@ Require Import LjsSyntax.
 Require Import String.
 Require Import LibStream.
 
-Module Heap := HeapUtils.Heap.
+Implicit Type st : store.
+Implicit Type e : expr.
+Implicit Type v : value.
+Implicit Type loc : value_loc.
+Implicit Type c : ctx.
+Implicit Type ptr : object_ptr.
+Implicit Type obj : object.
 
 (* LambdaJS environment storage. *)
 
-Definition add_value (st : store) (val : value) : (store * value_loc) :=
+Definition add_value st v : (store * value_loc) :=
   match st with
   | store_intro obj_heap val_heap (loc ::: stream) =>
-    (store_intro obj_heap (Heap.write val_heap loc val) stream, loc)
+    (store_intro obj_heap (Heap.write val_heap loc v) stream, loc)
   end
 .
-Fixpoint add_values (st : store) (vals : list value) : store * list value_loc :=
+Fixpoint add_values st (vals : list value) : store * list value_loc :=
   match vals with
   | nil => (st, nil)
   | val :: vals => 
@@ -24,7 +30,7 @@ Fixpoint add_values (st : store) (vals : list value) : store * list value_loc :=
     end
   end
 .
-Definition add_object (st : store) (obj : object) : (store * value) :=
+Definition add_object st obj : (store * value) :=
   match st with
   | store_intro obj_heap val_heap (ptr ::: stream) =>
     ((store_intro
@@ -34,37 +40,37 @@ Definition add_object (st : store) (obj : object) : (store * value) :=
     ), (value_object ptr))
   end
 .
-Definition add_closure (c : ctx) (st : store) args body : (store * value) :=
+Definition add_closure c st args body : (store * value) :=
   match st with
   | store_intro obj_heap val_heap (id ::: stream) =>
     (store_intro obj_heap val_heap stream, value_closure id c args body)
   end
 .
-Definition add_value_at_location (st : store) (loc : value_loc) (val : value) : store :=
+Definition add_value_at_location st loc v : store :=
   (* TODO: Remove the old value from the Heap (or fix LibHeap to prevent duplicates) *)
   match st with
-  | store_intro obj_heap val_heap stream => (store_intro obj_heap (Heap.write val_heap loc val) stream)
+  | store_intro obj_heap val_heap stream => (store_intro obj_heap (Heap.write val_heap loc v) stream)
   end
 .
-Definition add_named_location (c : ctx) (name : id) (loc : value_loc) : ctx :=
+Definition add_named_location c i loc : ctx :=
   match c with
   | ctx_intro loc_heap =>
-    ctx_intro (Heap.write loc_heap name loc) 
+    ctx_intro (Heap.write loc_heap i loc) 
   end
 .
-Definition add_named_value_loc (c : ctx) (st : store) (name : id) (val : value) : (ctx * store * value_loc) :=
+Definition add_named_value_loc c st i v : (ctx * store * value_loc) :=
   match c, st with
   | ctx_intro loc_heap, store_intro obj_heap val_heap (loc ::: stream) => 
-    (ctx_intro (Heap.write loc_heap name loc), store_intro obj_heap (Heap.write val_heap loc val) stream, loc)
+    (ctx_intro (Heap.write loc_heap i loc), store_intro obj_heap (Heap.write val_heap loc v) stream, loc)
   end
 .
-Definition add_named_value (c : ctx) (st : store) (name : id) (val : value) : ctx * store := 
-  match add_named_value_loc c st name val with (c', st', _) => (c', st') end
+Definition add_named_value c st i v : ctx * store := 
+  match add_named_value_loc c st i v with (c', st', _) => (c', st') end
 .
-Definition update_object (st : store) (ptr : object_ptr) (new_obj : object) : store :=
+Definition update_object st ptr obj : store :=
   (* TODO: Remove the old object from the Heap (or fix LibHeap to prevent duplicates) *)
   match st with
-  | store_intro obj_heap val_heap stream => (store_intro (Heap.write obj_heap ptr new_obj) val_heap stream)
+  | store_intro obj_heap val_heap stream => (store_intro (Heap.write obj_heap ptr obj) val_heap stream)
   end
 .
 
@@ -77,14 +83,20 @@ Definition add_option_value st (oval : option value) : (store * option value_loc
 Definition add_bool st (b : bool) : (store * value_loc) :=
   add_value st (if b then value_true else value_false)
 .
-Definition get_object (st : store) (ptr : object_ptr) : option object :=
+Definition get_object st ptr : option object :=
   Heap.read_option (object_heap st) ptr
 .
-Definition get_value (st : store) (loc : value_loc) : option value :=
+Definition get_value st loc : option value :=
   Heap.read_option (value_heap st) loc
 .
-Definition get_loc  (c : ctx) (name : id) : option value_loc :=
-  Heap.read_option (loc_heap c) name
+Definition get_loc c i : option value_loc :=
+  Heap.read_option (loc_heap c) i
+.
+Definition object_binds st ptr obj :=
+  Heap.binds (object_heap st) ptr obj
+.
+Definition value_binds st loc v :=
+  Heap.binds (value_heap st) loc v
 .
 
 (* Returns the value associated to a variable name (aka. id) in the current
@@ -96,10 +108,10 @@ Definition get_value_of_name c store (name : id) : option value :=
   end
 .
 
-Definition num_objects (st : store) : nat :=
+Definition num_objects st : nat :=
   List.length (Heap.to_list (object_heap st)).
 
-Definition num_values (st : store) : nat :=
+Definition num_values st : nat :=
   List.length (Heap.to_list (value_heap st)).
 
 Definition envstore_of_obj_aux (o : option (ctx * store)) (p : string * attributes) : option (ctx * store) :=
