LambdaS5/coq/LjsCompleteness.v
@@ -1,0 +1,388 @@
+Generalizable All Variables.
+Set Implicit Arguments.
+Require Import LjsShared.
+Require Import Utils.
+Require Import LjsSyntax.
+Require Import LjsPrettyInterm.
+Require Import LjsPrettyRules.
+Require Import LjsPrettyRulesIndexed.
+Require Import LjsStore.
+Require Import LjsCommon.
+Require Import LjsValues.
+Require Import LjsOperators.
+Require Import LjsMonads.
+Require Import LjsInterpreter.
+Require Import JsNumber.
+Require Import Coq.Strings.String.
+
+Import ListNotations.
+
+Open Scope list_scope.
+
+Implicit Type A B : Type.
+Implicit Type runs : runs_type.
+Implicit Type st : store.
+Implicit Type e : expr.
+Implicit Type v : value.
+Implicit Type loc : value_loc.
+Implicit Type s : string.
+Implicit Type n : number.
+Implicit Type i : id.
+Implicit Type o : out.
+Implicit Type c : ctx.
+Implicit Type ptr : object_ptr.
+Implicit Type obj : object.
+Implicit Type re : result.
+Implicit Type r : res.
+
+Lemma assert_get_loc_lemma : forall {A c i loc} cont, get_loc c i = Some loc -> @assert_get_loc A c i cont = cont loc.
+Proof.
+    introv H. unfolds. rewrite H. reflexivity.
+Qed.
+
+Lemma assert_deref_lemma : forall {A st loc v} cont, get_value st loc = Some v -> @assert_deref A st loc cont = cont v.
+Proof.
+    introv H. unfolds. rewrite H. reflexivity.
+Qed.
+
+Lemma eval_cont_lemma : forall {A runs c st e re} cont,
+    runs_type_eval runs c st e = re ->
+    @eval_cont A runs c st e cont = cont re.
+Proof.
+    introv H. unfolds. rewrite H. reflexivity.
+Qed.
+
+Lemma if_eval_return_lemma : forall {runs c st st' e v} cont, 
+    runs_type_eval runs c st e = result_some (out_ter st' (res_value v)) ->
+    if_eval_return runs c st e cont = cont st' v.
+Proof.
+    introv H. unfolds. lets L : @eval_cont_lemma H. rewrite L. reflexivity.
+Qed.
+
+Lemma assert_get_object_ptr_lemma : forall {A ptr} cont, 
+    @assert_get_object_ptr A (value_object ptr) cont = cont ptr.
+Proof.
+    intros. reflexivity.
+Qed.
+
+Lemma assert_get_object_from_ptr_lemma : forall {A st ptr obj} cont, 
+    get_object st ptr = Some obj -> @assert_get_object_from_ptr A st ptr cont = cont obj.
+Proof.
+    introv H. unfolds. rewrite H. reflexivity.
+Qed.
+
+Lemma assert_get_object_lemma : forall {A st ptr obj} cont, 
+    get_object st ptr = Some obj -> @assert_get_object A st (value_object ptr) cont = cont obj.
+Proof.
+    introv H. unfolds. rewrite assert_get_object_ptr_lemma. 
+    auto using assert_get_object_from_ptr_lemma.
+Qed.
+
+Lemma assert_get_string_lemma : forall {A s} cont, 
+    @assert_get_string A (value_string s) cont = cont s.
+Proof.
+    intros. reflexivity.
+Qed.
+
+Lemma assert_get_bool_lemma : forall {A v b} cont,
+    value_to_bool v = Some b -> @assert_get_bool A v cont = cont b.
+Proof.
+    introv H. unfolds. destruct v; inverts H; reflexivity.
+Qed.
+
+Lemma assert_get_bool_false_lemma : forall {A} cont,
+    @assert_get_bool A value_false cont = cont false.
+Proof.
+    intros. reflexivity.
+Qed.
+
+Lemma assert_get_bool_true_lemma : forall {A} cont,
+    @assert_get_bool A value_true cont = cont true.
+Proof.
+    intros. reflexivity.
+Qed.
+
+Lemma if_result_some_lemma : forall {A B res a} cont,
+    res = result_some a -> @if_result_some A B res cont = cont a.
+Proof.
+    introv H. rewrite H. reflexivity.
+Qed.
+
+Lemma change_object_cont_lemma : forall {st ptr obj} cont, 
+    get_object st ptr = Some obj -> 
+    change_object_cont st ptr cont = cont obj (fun st new_obj ret =>
+        result_some (out_ter (LjsStore.update_object st ptr new_obj) (res_value ret))).
+Proof.
+    introv H. unfolds. rewrite H. reflexivity.
+Qed.
+
+Ltac ljs_eval :=
+    match goal with
+    | H : get_loc ?c ?i = Some _ |- assert_get_loc ?c ?i _ = _ => rewrite (assert_get_loc_lemma _ H)
+    | H : get_value ?st ?loc = Some _ |- assert_deref ?st ?loc _ = _ => rewrite (assert_deref_lemma _ H)
+    | H : runs_type_eval ?runs ?c ?st ?e = _ |- eval_cont ?runs ?c ?st ?e _ = _ => rewrite (eval_cont_lemma _ H)
+    | H : runs_type_eval ?runs ?c ?st ?e = result_some (out_ter _ (res_value _)) 
+        |- if_eval_return ?runs ?c ?st ?e _ = _ => rewrite (if_eval_return_lemma _ H)
+    | H : get_object ?st ?ptr = Some _ |- assert_get_object_from_ptr ?st ?ptr _ = _ => 
+        rewrite (assert_get_object_from_ptr_lemma _ H)
+    | H : get_object ?st ?ptr = Some _ |- assert_get_object ?st (value_object ?ptr) _ = _ => 
+        rewrite (assert_get_object_lemma _ H)
+    | H : get_object ?st ?ptr = Some _ |- change_object_cont ?st ?ptr _ = _ => 
+        rewrite (change_object_cont_lemma _ H)
+    | H : value_to_bool ?v = Some _ |- assert_get_bool ?v _ = _ => rewrite (assert_get_bool_lemma _ H)
+    | |- assert_get_bool value_true _ = _ => rewrite (assert_get_bool_true_lemma _)
+    | |- assert_get_bool value_false _ = _ => rewrite (assert_get_bool_false_lemma _)
+    | |- assert_get_string (value_string _) _ = _ => rewrite (assert_get_string_lemma _)
+    | |- assert_get_object_ptr (value_object _) _ = _ => rewrite (assert_get_object_ptr_lemma _)
+    | H : ?res = result_some _ |- if_result_some ?res _ = _ => rewrite (if_result_some_lemma _ H)
+(*
+    | |- result_value _ _ = _ => reflexivity
+    | |- result_exception _ _ = _ => reflexivity
+    | |- result_break _ _ = _ => reflexivity
+    | |- ?x = ?x => reflexivity
+*)
+    end.
+
+Lemma if_value_abort_lemma : forall {o} cont,
+    abort o ->
+    if_value (result_some o) cont = result_some o.
+Proof.
+    introv HA. inversion HA as [ | st r HC ].
+    reflexivity.
+    inversion HC; reflexivity. 
+Qed.
+
+Lemma is_eval_return_abort_lemma : forall {runs c st e o} cont,
+    abort o ->
+    runs_type_eval runs c st e = result_some o ->
+    if_eval_return runs c st e cont = result_some o.
+Proof.
+    introv HA H. unfolds. lets L : @eval_cont_lemma H. rewrite L.
+    applys @if_value_abort_lemma HA.
+Qed.
+
+Ltac ljs_abort :=
+    match goal with
+    | H : abort ?o |- if_value (result_some ?o) _ = result_some ?o => apply (if_value_abort_lemma _ H)
+    | H : abort ?o, H1 : runs_type_eval ?runs ?c ?st ?e = result_some ?o 
+        |- if_eval_return ?runs ?c ?st ?e ?cont = result_some ?o => apply (is_eval_return_abort_lemma _ H H1)
+    end. 
+
+Lemma lazyruns_lemma : forall runs, suspend_runs (fun _ => runs) = runs.
+Proof.
+    intros.
+    destruct runs. unfolds.
+    autorewrite with rew_eta. 
+    reflexivity.
+Qed.
+
+Lemma eval_runs_geq : forall e c st o (n1 n2 : nat), 
+    n1 <= n2 -> runs_type_eval (runs n1) c st e = result_some o -> 
+    runs_type_eval (runs n2) c st e = result_some o. 
+Proof.
+    (* TODO *)
+Admitted.
+
+(*
+Ltac injects := 
+    match goal with
+    | H : (_, _) = (_, _) |- _ => injection H; clear H
+    | H : Some _ = Some _ |- _ => injection H; clear H
+    end.
+*)
+
+Ltac ljs_specialize_ih H1 :=
+    match goal with
+    | H : red_exprh _ _ _ _ _, IH : forall c st e o, red_exprh _ _ _ _ _ -> _ |- _ => 
+        lets H1 : IH H; clear H
+    end.
+
+Tactic Notation "ljs_specialize_ih" :=
+    let H := fresh "H" in ljs_specialize_ih H.
+
+Ltac ljs_inv_red :=
+    match goal with
+    | H	: red_exprh _ _ _ _ _ |- _ => 
+        inverts H
+    end.
+
+Ltac ljs_inv_red_internal :=
+    match goal with
+    | H	: red_exprh _ _ _ ?e _ |- _ => 
+        match e with 
+        | expr_basic _ => fail 
+        | _ => inverts H
+        end
+    end.
+
+Ltac ljs_inv_red_abort := ljs_inv_red_internal; [ | ljs_abort].
+
+Lemma exists_S : forall (P : nat -> Prop), (exists k, P (S k)) -> exists k, P k.
+Proof.
+    introv H.
+    destruct H as (k&H).
+    eexists; eassumption.
+Qed.
+
+Ltac ljs_eval_step := ljs_specialize_ih; ljs_inv_red_abort; ljs_eval.
+(*
+Ltac ljs_eval_push := ljs_eval_step || ljs_eval.
+*)
+Ltac ljs_eval_push := ljs_specialize_ih || ljs_inv_red_abort || ljs_eval || reflexivity || assumption.
+
+Lemma object_properties_lemma : forall k,
+    (forall c st e o, red_exprh k c st e o -> runs_type_eval (runs k) c st e = result_some o) -> 
+    forall l c st obj o,
+    red_exprh k c st (expr_object_6 obj l) o ->
+    eval_object_properties (runs k) c st l obj (fun st obj =>
+                  let (st, loc) := add_object st obj
+                  in result_value st loc
+          ) = result_some o.
+Proof.
+    introv IH.
+    induction l as [|p l]; introv R.
+    (* [] *)
+    simpl.
+    ljs_inv_red.
+    cases_let.
+    injects.
+    reflexivity.
+    (* [] *)
+    destruct p as (i&[()|()]); ljs_inv_red; simpl.
+    (* data *)
+    repeat ljs_eval_push.
+    eauto.
+    (* accessor *)
+    repeat ljs_eval_push.
+    eauto.
+Qed.
+
+Lemma eval_complete_lemma : forall k c st e o,
+    red_exprh k c st e o -> runs_type_eval (runs k) c st e = result_some o.
+Proof.
+    induction k; 
+    introv R;
+    inverts R;
+    simpls.
+    (* null *)
+    reflexivity.
+    (* undefined *)
+    reflexivity.
+    (* string *)
+    reflexivity.
+    (* number *)
+    reflexivity.
+    (* true *)
+    reflexivity.
+    (* false *)
+    reflexivity.
+    (* id *)
+    unfolds. 
+    repeat ljs_eval; reflexivity.
+    (* lambda *)
+    unfolds.
+    cases_let. injects. reflexivity.
+    (* object *)
+    repeat ljs_eval_push.
+    eauto using object_properties_lemma.
+    (* get_attr *)
+    unfolds.
+    repeat ljs_eval_push.
+    (* set_attr *)
+    unfolds.
+    repeat ljs_eval_push.
+    (* get_obj_attr *)
+    unfolds.
+    repeat ljs_eval_push.
+    (* set_obj_attr *)
+    unfolds.
+    repeat ljs_eval_push.
+    (* get_field *)
+    unfolds.
+    repeat ljs_eval_push.
+    destruct oattr as [[|]|].
+    ljs_inv_red. reflexivity.
+    skip.
+    ljs_inv_red. reflexivity.
+    (* set_field *)
+    unfolds.
+    repeat ljs_eval_push.
+    unfold change_object_property, change_object_property_cont.
+    destruct oattr as [[|]|].
+    repeat (ljs_eval || cases_if || cases_match_option); ljs_inv_red; tryfalse; reflexivity.
+    skip.
+    cases_if; ljs_inv_red; tryfalse; try ljs_eval; reflexivity.
+    (* delete_field *)
+    unfolds.
+    repeat ljs_eval_push.
+    repeat (ljs_eval || cases_if || cases_match_option); ljs_inv_red; tryfalse; reflexivity.
+    (* own_field_names *)
+    unfolds.
+    repeat ljs_eval_push.
+    cases_let.
+    injects.
+    reflexivity.
+    (* set_bang *)
+    unfolds.
+    repeat ljs_eval_push.
+    (* op1 *)
+    unfolds.
+    repeat ljs_eval_push.
+    (* op2 *)
+    unfolds.
+    repeat ljs_eval_push.
+    (* if *)
+    unfolds.
+    ljs_specialize_ih. ljs_inv_red_internal.
+    ljs_specialize_ih.
+    repeat ljs_eval_push.
+    ljs_specialize_ih.
+    repeat ljs_eval_push.
+    ljs_abort.
+    (* app *)
+    unfolds.
+    repeat ljs_eval_push.
+    skip.
+    (* seq *)
+    unfolds.
+    repeat ljs_eval_push.
+    (* let *)
+    unfolds.
+    repeat ljs_eval_push.
+    cases_let.
+    injects.
+    repeat ljs_eval_push.
+    (* rec *)
+    unfolds.
+    repeat ljs_eval_push.
+    cases_let.
+    injects.
+    repeat ljs_eval_push.
+    (* label *)
+    unfolds.
+    repeat ljs_eval_push.
+    skip.
+    (* break *)
+    unfolds.
+    repeat ljs_eval_push.
+    (* trycatch *)
+    unfolds.
+    repeat ljs_eval_push.
+    skip.
+    (* tryfinally *)
+    unfolds.
+    repeat ljs_eval_push.
+    skip.
+    (* throw *)
+    unfolds.
+    repeat ljs_eval_push.
+    (* eval *)
+    unfolds.
+    repeat ljs_eval_push.
+    repeat cases_match_option.
+    cases_let.
+    repeat injects.
+    repeat ljs_eval_push.
+    (* hint *)
+    repeat ljs_eval_push.
+Qed.
