LambdaS5/coq/LjsPrettyRulesIndexed.v
@@ -1,0 +1,599 @@
+Generalizable All Variables.
+Set Implicit Arguments.
+Require Import LjsShared.
+Require Import LjsSyntax.
+Require Import LjsPrettyInterm.
+Require Import LjsStore.
+Require Import LjsCommon.
+Require Import LjsValues.
+Require Import LjsOperators.
+Require Import LjsMonads.
+Require Import JsNumber.
+Require Import Coq.Strings.String.
+Import List.ListNotations.
+
+Open Scope list_scope.
+
+Implicit Type st : store.
+Implicit Type e : expr.
+Implicit Type v : value.
+Implicit Type loc : value_loc.
+Implicit Type s : string.
+Implicit Type n : number.
+Implicit Type i : id.
+Implicit Type o : out.
+Implicit Type c : ctx.
+Implicit Type ptr : object_ptr.
+Implicit Type obj : object.
+
+Inductive red_exprh : nat -> ctx -> store -> ext_expr -> out -> Prop :=
+| red_exprh_null : forall k c st, red_exprh (S k) c st expr_null (out_ter st (res_value value_null))
+| red_exprh_undefined : forall k c st, red_exprh (S k) c st expr_undefined (out_ter st (res_value value_undefined))
+| red_exprh_string : forall k c st s, red_exprh (S k) c st (expr_string s) (out_ter st (res_value (value_string s)))
+| red_exprh_number : forall k c st n, red_exprh (S k) c st (expr_number n) (out_ter st (res_value (value_number n)))
+| red_exprh_true : forall k c st, red_exprh (S k) c st expr_true (out_ter st (res_value value_true))
+| red_exprh_false : forall k c st, red_exprh (S k) c st expr_false (out_ter st (res_value value_false))
+| red_exprh_id : forall k c st i loc v, 
+    get_loc c i = Some loc -> 
+    get_value st loc = Some v -> 
+    red_exprh (S k) c st (expr_id i) (out_ter st (res_value v))
+| red_exprh_lambda : forall k c st st' args body v,
+    (st', v) = add_closure c st args body ->
+    red_exprh (S k) c st (expr_lambda args body) (out_ter st' (res_value v))
+
+(* object *)
+| red_exprh_object : forall k c st e1 e2 e3 e4 e5 a o o',
+    red_exprh k c st e1 o ->
+    red_exprh k c st (expr_object_1 o e2 e3 e4 e5 a) o' ->
+    red_exprh (S k) c st (expr_object (objattrs_intro e1 e2 e3 e4 e5) a) o'
+| red_exprh_object_1 : forall k c st' st v1 e2 e3 e4 e5 a o o',
+    red_exprh k c st e2 o ->
+    red_exprh k c st (expr_object_2 v1 o e3 e4 e5 a) o' ->
+    red_exprh k c st' (expr_object_1 (out_ter st (res_value v1)) e2 e3 e4 e5 a) o'
+| red_exprh_object_1_abort : forall k c st e2 e3 e4 e5 a o,
+    abort o ->
+    red_exprh k c st (expr_object_1 o e2 e3 e4 e5 a) o
+| red_exprh_object_2 : forall k c st' st v1 v2 e3 e4 e5 a o o',
+    red_exprh k c st e3 o ->
+    red_exprh k c st (expr_object_3 v1 v2 o e4 e5 a) o' ->
+    red_exprh k c st' (expr_object_2 v1 (out_ter st (res_value v2)) e3 e4 e5 a) o'
+| red_exprh_object_2_abort : forall k c st v1 e3 e4 e5 a o,
+    abort o ->
+    red_exprh k c st (expr_object_2 v1 o e3 e4 e5 a) o
+| red_exprh_object_3 : forall k c st' st v1 v2 v3 e4 e5 a o o',
+    red_exprh k c st e4 o ->
+    red_exprh k c st (expr_object_4 v1 v2 v3 o e5 a) o' ->
+    red_exprh k c st' (expr_object_3 v1 v2 (out_ter st (res_value v3)) e4 e5 a) o'
+| red_exprh_object_3_abort : forall k c st v1 v2 e4 e5 a o,
+    abort o ->
+    red_exprh k c st (expr_object_3 v1 v2 o e4 e5 a) o
+| red_exprh_object_4 : forall k c st' st v1 v2 v3 v4 e5 a o o',
+    red_exprh k c st e5 o ->
+    red_exprh k c st (expr_object_5 v1 v2 v3 v4 o a) o' ->
+    red_exprh k c st' (expr_object_4 v1 v2 v3 (out_ter st (res_value v4)) e5 a) o'
+| red_exprh_object_4_abort : forall k c st v1 v2 v3 e5 a o,
+    abort o ->
+    red_exprh k c st (expr_object_4 v1 v2 v3 o e5 a) o
+| red_exprh_object_5 : forall k c st' st class extv ext proto code prim a o,
+    value_to_bool extv = Some ext ->
+    red_exprh k c st (expr_object_6 (object_intro proto class ext prim Heap.empty code) a) o ->
+    red_exprh k c st' (expr_object_5 (value_string class) extv proto code (out_ter st (res_value prim)) a) o
+| red_exprh_object_5_abort : forall k c st v1 v2 v3 v4 a o,
+    abort o ->
+    red_exprh k c st (expr_object_5 v1 v2 v3 v4 o a) o
+| red_exprh_object_6 : forall k c st st1 obj v,
+    (st1, v) = add_object st obj ->
+    red_exprh k c st (expr_object_6 obj nil) (out_ter st1 (res_value v))
+| red_exprh_object_6_data : forall k c st obj s e1 e2 e3 e4 a o o',
+    red_exprh k c st e1 o ->
+    red_exprh k c st (expr_object_data_1 obj a s o e2 e3 e4) o' ->
+    red_exprh k c st (expr_object_6 obj ((s, property_data (data_intro e3 e4 e2 e1)) :: a)) o'
+| red_exprh_object_data_1 : forall k c st' st obj a s v1 e2 e3 e4 o o',
+    red_exprh k c st e2 o ->
+    red_exprh k c st (expr_object_data_2 obj a s v1 o e3 e4) o' ->
+    red_exprh k c st' (expr_object_data_1 obj a s (out_ter st (res_value v1)) e2 e3 e4) o'
+| red_exprh_object_data_1_abort : forall k c st obj a s e2 e3 e4 o,
+    abort o ->
+    red_exprh k c st (expr_object_data_1 obj a s o e2 e3 e4) o
+| red_exprh_object_data_2 : forall k c st' st obj a s v1 v2 e3 e4 o o',
+    red_exprh k c st e3 o ->
+    red_exprh k c st (expr_object_data_3 obj a s v1 v2 o e4) o' ->
+    red_exprh k c st' (expr_object_data_2 obj a s v1 (out_ter st (res_value v2)) e3 e4) o'
+| red_exprh_object_data_2_abort : forall k c st obj a s v1 e3 e4 o,
+    abort o ->
+    red_exprh k c st (expr_object_data_2 obj a s v1 o e3 e4) o
+| red_exprh_object_data_3 : forall k c st' st obj a s v1 v2 v3 e4 o o',
+    red_exprh k c st e4 o ->
+    red_exprh k c st (expr_object_data_4 obj a s v1 v2 v3 o) o' ->
+    red_exprh k c st' (expr_object_data_3 obj a s v1 v2 (out_ter st (res_value v3)) e4) o'
+| red_exprh_object_data_3_abort : forall k c st obj a s v1 v2 e4 o,
+    abort o ->
+    red_exprh k c st (expr_object_data_3 obj a s v1 v2 o e4) o
+| red_exprh_object_data_4 : forall k c st' st obj a s v1 v2 v3 v4 b1 b2 b4 o,
+    value_to_bool v1 = Some b1 ->
+    value_to_bool v2 = Some b2 ->
+    value_to_bool v4 = Some b4 ->
+    red_exprh k c st (expr_object_6 (set_object_property obj s (attributes_data_of (attributes_data_intro v3 b4 b2 b1))) a) o ->
+    red_exprh k c st' (expr_object_data_4 obj a s v1 v2 v3 (out_ter st (res_value v4))) o
+| red_exprh_object_data_4_abort : forall k c st obj a s v1 v2 v3 o,
+    abort o ->
+    red_exprh k c st (expr_object_data_4 obj a s v1 v2 v3 o) o
+| red_exprh_object_6_accessor : forall k c st obj s e1 e2 e3 e4 a o o',
+    red_exprh k c st e1 o ->
+    red_exprh k c st (expr_object_accessor_1 obj a s o e2 e3 e4) o' ->
+    red_exprh k c st (expr_object_6 obj ((s, property_accessor (accessor_intro e3 e4 e2 e1)) :: a)) o'
+| red_exprh_object_accessor_1 : forall k c st' st obj a s v1 e2 e3 e4 o o',
+    red_exprh k c st e2 o ->
+    red_exprh k c st (expr_object_accessor_2 obj a s v1 o e3 e4) o' ->
+    red_exprh k c st' (expr_object_accessor_1 obj a s (out_ter st (res_value v1)) e2 e3 e4) o'
+| red_exprh_object_accessor_1_abort : forall k c st obj a s e2 e3 e4 o,
+    abort o ->
+    red_exprh k c st (expr_object_accessor_1 obj a s o e2 e3 e4) o
+| red_exprh_object_accessor_2 : forall k c st' st obj a s v1 v2 e3 e4 o o',
+    red_exprh k c st e3 o ->
+    red_exprh k c st (expr_object_accessor_3 obj a s v1 v2 o e4) o' ->
+    red_exprh k c st' (expr_object_accessor_2 obj a s v1 (out_ter st (res_value v2)) e3 e4) o'
+| red_exprh_object_accessor_2_abort : forall k c st obj a s v1 e3 e4 o,
+    abort o ->
+    red_exprh k c st (expr_object_accessor_2 obj a s v1 o e3 e4) o
+| red_exprh_object_accessor_3 : forall k c st' st obj a s v1 v2 v3 e4 o o',
+    red_exprh k c st e4 o ->
+    red_exprh k c st (expr_object_accessor_4 obj a s v1 v2 v3 o) o' ->
+    red_exprh k c st' (expr_object_accessor_3 obj a s v1 v2 (out_ter st (res_value v3)) e4) o'
+| red_exprh_object_accessor_3_abort : forall k c st obj a s v1 v2 e4 o,
+    abort o ->
+    red_exprh k c st (expr_object_accessor_3 obj a s v1 v2 o e4) o
+| red_exprh_object_accessor_4 : forall k c st' st obj a s v1 v2 v3 v4 b1 b2 o,
+    value_to_bool v1 = Some b1 ->
+    value_to_bool v2 = Some b2 ->
+    red_exprh k c st (expr_object_6 (set_object_property obj s (attributes_accessor_of (attributes_accessor_intro v3 v4 b2 b1))) a) o ->
+    red_exprh k c st' (expr_object_accessor_4 obj a s v1 v2 v3 (out_ter st (res_value v4))) o
+| red_exprh_object_accessor_4_abort : forall k c st obj a s v1 v2 v3 o,
+    abort o ->
+    red_exprh k c st (expr_object_accessor_4 obj a s v1 v2 v3 o) o
+
+(* get_attr *)
+| red_exprh_get_attr : forall k c st pa e1 e2 o o',
+    red_exprh k c st e1 o ->
+    red_exprh k c st (expr_get_attr_1 pa o e2) o' ->
+    red_exprh (S k) c st (expr_get_attr pa e1 e2) o'
+| red_exprh_get_attr_1 : forall k c st' st pa v1 e2 o o',
+    red_exprh k c st e2 o ->
+    red_exprh k c st (expr_get_attr_2 pa v1 o) o' ->
+    red_exprh k c st' (expr_get_attr_1 pa (out_ter st (res_value v1)) e2) o'
+| red_exprh_get_attr_1_abort : forall k c st pa e2 o,
+    abort o ->
+    red_exprh k c st (expr_get_attr_1 pa o e2) o
+| red_exprh_get_attr_2 : forall k c st' st pa s ptr obj v,
+    get_object st ptr = Some obj ->
+    get_object_pattr obj s pa = result_some v ->
+    red_exprh k c st' (expr_get_attr_2 pa (value_object ptr) (out_ter st (res_value (value_string s)))) (out_ter st (res_value v))
+| red_exprh_get_attr_2_abort : forall k c st pa v1 o,
+    abort o ->
+    red_exprh k c st (expr_get_attr_2 pa v1 o) o
+
+(* set_attr *)
+| red_exprh_set_attr : forall k c st pa e1 e2 e3 o o',
+    red_exprh k c st e1 o ->
+    red_exprh k c st (expr_set_attr_1 pa o e2 e3) o' ->
+    red_exprh (S k) c st (expr_set_attr pa e1 e2 e3) o'
+| red_exprh_set_attr_1 : forall k c st' st pa v1 e2 e3 o o',
+    red_exprh k c st e2 o ->
+    red_exprh k c st (expr_set_attr_2 pa v1 o e3) o' ->
+    red_exprh k c st' (expr_set_attr_1 pa (out_ter st (res_value v1)) e2 e3) o'
+| red_exprh_set_attr_1_abort : forall k c st pa e2 e3 o,
+    abort o ->
+    red_exprh k c st (expr_set_attr_1 pa o e2 e3) o
+| red_exprh_set_attr_2 : forall k c st' st pa v1 v2 e3 o o',
+    red_exprh k c st e3 o ->
+    red_exprh k c st (expr_set_attr_3 pa v1 v2 o) o' ->
+    red_exprh k c st' (expr_set_attr_2 pa v1 (out_ter st (res_value v2)) e3) o'
+| red_exprh_set_attr_2_abort : forall k c st pa v1 e3 o,
+    abort o ->
+    red_exprh k c st (expr_set_attr_2 pa v1 o e3) o
+| red_exprh_set_attr_3 : forall k c st' st st1 pa ptr obj obj' s v,
+    get_object st ptr = Some obj ->
+    set_object_pattr obj s pa v = result_some obj' ->
+    st1 = update_object st ptr obj' ->
+    red_exprh k c st' (expr_set_attr_3 pa (value_object ptr) (value_string s) (out_ter st (res_value v))) (out_ter st1 (res_value v))
+| red_exprh_set_attr_3_abort : forall k c st pa v1 v2 o,
+    abort o ->
+    red_exprh k c st (expr_set_attr_3 pa v1 v2 o) o
+
+(* get_obj_attr *)
+| red_exprh_get_obj_attr : forall k c st oa e1 o o',
+    red_exprh k c st e1 o ->
+    red_exprh k c st (expr_get_obj_attr_1 oa o) o' ->
+    red_exprh (S k) c st (expr_get_obj_attr oa e1) o'
+| red_exprh_get_obj_attr_1 : forall k c st' st oa ptr obj,
+    get_object st ptr = Some obj ->
+    red_exprh k c st' (expr_get_obj_attr_1 oa (out_ter st (res_value (value_object ptr)))) (out_ter st (res_value (get_object_oattr obj oa)))
+| red_exprh_get_obj_attr_1_abort : forall k c st oa o,
+    abort o ->
+    red_exprh k c st (expr_get_obj_attr_1 oa o) o
+
+(* set_obj_attr *)
+| red_exprh_set_obj_attr : forall k c st oa e1 e2 o o',
+    red_exprh k c st e1 o ->
+    red_exprh k c st (expr_set_obj_attr_1 oa o e2) o' ->
+    red_exprh (S k) c st (expr_set_obj_attr oa e1 e2) o'
+| red_exprh_set_obj_attr_1 : forall k c st' st oa v1 e2 o o',
+    red_exprh k c st e2 o ->
+    red_exprh k c st (expr_set_obj_attr_2 oa v1 o) o' ->
+    red_exprh k c st' (expr_set_obj_attr_1 oa (out_ter st (res_value v1)) e2) o'
+| red_exprh_set_obj_attr_1_abort : forall k c st oa e2 o,
+    abort o ->
+    red_exprh k c st (expr_set_obj_attr_1 oa o e2) o
+| red_exprh_set_obj_attr_2 : forall k c st' st st1 oa ptr obj obj' v,
+    get_object st ptr = Some obj ->
+    set_object_oattr obj oa v = result_some obj' ->
+    st1 = update_object st ptr obj' ->
+    red_exprh k c st' (expr_set_obj_attr_2 oa (value_object ptr) (out_ter st (res_value v))) (out_ter st1 (res_value v))
+| red_exprh_set_obj_attr_2_abort : forall k c st oa v1 o,
+    abort o ->
+    red_exprh k c st (expr_set_obj_attr_2 oa v1 o) o
+
+(* get_field *)
+| red_exprh_get_field : forall k c st e1 e2 e3 o o',
+    red_exprh k c st e1 o ->
+    red_exprh k c st (expr_get_field_1 o e2 e3) o' ->
+    red_exprh (S k) c st (expr_get_field e1 e2 e3) o'
+| red_exprh_get_field_1 : forall k c st' st v1 e2 e3 o o',
+    red_exprh k c st e2 o ->
+    red_exprh k c st (expr_get_field_2 v1 o e3) o' ->
+    red_exprh k c st' (expr_get_field_1 (out_ter st (res_value v1)) e2 e3) o'
+| red_exprh_get_field_1_abort : forall k c st e2 e3 o,
+    abort o ->
+    red_exprh k c st (expr_get_field_1 o e2 e3) o
+| red_exprh_get_field_2 : forall k c st' st v1 v2 e3 o o',
+    red_exprh k c st e3 o ->
+    red_exprh k c st (expr_get_field_3 v1 v2 o) o' ->
+    red_exprh k c st' (expr_get_field_2 v1 (out_ter st (res_value v2)) e3) o'
+| red_exprh_get_field_2_abort : forall k c st v1 e3 o,
+    abort o ->
+    red_exprh k c st (expr_get_field_2 v1 o e3) o
+| red_exprh_get_field_3 : forall k c st' st v3 ptr s oattr o,
+    get_property st ptr s = result_some oattr ->
+    red_exprh k c st (expr_get_field_4 ptr oattr v3) o ->
+    red_exprh k c st' (expr_get_field_3 (value_object ptr) (value_string s) (out_ter st (res_value v3))) o
+| red_exprh_get_field_3_abort : forall k c st v1 v2 o,
+    abort o ->
+    red_exprh k c st (expr_get_field_3 v1 v2 o) o
+| red_exprh_get_field_4_no_field : forall k c st ptr v3,
+    red_exprh k c st (expr_get_field_4 ptr None v3) (out_ter st (res_value value_undefined))
+| red_exprh_get_field_4_get_field : forall k c st ptr v3 data,
+    red_exprh k c st (expr_get_field_4 ptr (Some (attributes_data_of data)) v3) (out_ter st (res_value (attributes_data_value data)))
+| red_exprh_get_field_4_getter : forall k c st ptr v3 acc o,
+    red_exprh k c st (expr_app_2 (attributes_accessor_get acc) [v3; value_object ptr] nil) o ->
+    red_exprh k c st (expr_get_field_4 ptr (Some (attributes_accessor_of acc)) v3) o
+
+(* set_field *)
+| red_exprh_set_field : forall k c st e1 e2 e3 e4 o o',
+    red_exprh k c st e1 o ->
+    red_exprh k c st (expr_set_field_1 o e2 e3 e4) o' ->
+    red_exprh (S k) c st (expr_set_field e1 e2 e3 e4) o'
+| red_exprh_set_field_1 : forall k c st' st v1 e2 e3 e4 o o',
+    red_exprh k c st e2 o ->
+    red_exprh k c st (expr_set_field_2 v1 o e3 e4) o' ->
+    red_exprh k c st' (expr_set_field_1 (out_ter st (res_value v1)) e2 e3 e4) o'
+| red_exprh_set_field_1_abort : forall k c st e2 e3 e4 o,
+    abort o ->
+    red_exprh k c st (expr_set_field_1 o e2 e3 e4) o
+| red_exprh_set_field_2 : forall k c st' st v1 v2 e3 e4 o o',
+    red_exprh k c st e3 o ->
+    red_exprh k c st (expr_set_field_3 v1 v2 o e4) o' ->
+    red_exprh k c st' (expr_set_field_2 v1 (out_ter st (res_value v2)) e3 e4) o'
+| red_exprh_set_field_2_abort : forall k c st v1 e3 e4 o,
+    abort o ->
+    red_exprh k c st (expr_set_field_2 v1 o e3 e4) o
+| red_exprh_set_field_3 : forall k c st' st v1 v2 v3 e4 o o',
+    red_exprh k c st e4 o ->
+    red_exprh k c st (expr_set_field_4 v1 v2 v3 o) o' ->
+    red_exprh k c st' (expr_set_field_3 v1 v2 (out_ter st (res_value v3)) e4) o'
+| red_exprh_set_field_3_abort : forall k c st v1 v2 e4 o,
+    abort o ->
+    red_exprh k c st (expr_set_field_3 v1 v2 o e4) o
+| red_exprh_set_field_4 : forall k c st' st ptr obj oattr s v3 v4 o,
+    get_property st ptr s = result_some oattr ->
+    get_object st ptr = Some obj ->
+    red_exprh k c st (expr_set_field_5 ptr obj oattr s v3 v4) o ->
+    red_exprh k c st' (expr_set_field_4 (value_object ptr) (value_string s) v3 (out_ter st (res_value v4))) o
+| red_exprh_set_field_4_abort : forall k c st v1 v2 v3 o,
+    abort o ->
+    red_exprh k c st (expr_set_field_4 v1 v2 v3 o) o
+| red_exprh_set_field_5_set_field : forall k c st st1 ptr obj data s v3 v4,
+    get_object_property obj s <> None ->
+    attributes_data_writable data = true ->
+    st1 = update_object st ptr (set_object_property obj s (attributes_data_of (attributes_data_value_update data v3))) ->
+    red_exprh k c st (expr_set_field_5 ptr obj (Some (attributes_data_of data)) s v3 v4) (out_ter st1 (res_value v3))
+| red_exprh_set_field_5_shadow_field : forall k c st st1 ptr obj data s v3 v4,
+    get_object_property obj s = None ->
+    object_extensible obj = true ->
+    attributes_data_writable data = true ->
+    st1 = update_object st ptr (set_object_property obj s (attributes_data_of (attributes_data_intro v3 true true true))) ->
+    red_exprh k c st (expr_set_field_5 ptr obj (Some (attributes_data_of data)) s v3 v4) (out_ter st1 (res_value v3))
+| red_exprh_set_field_5_add_field : forall k c st st1 ptr obj s v3 v4,
+    object_extensible obj = true ->
+    st1 = update_object st ptr (set_object_property obj s (attributes_data_of (attributes_data_intro v3 true true true))) ->
+    red_exprh k c st (expr_set_field_5 ptr obj None s v3 v4) (out_ter st1 (res_value v3))
+| red_exprh_set_field_5_setter : forall k c st ptr obj acc s v3 v4 o,
+    red_exprh k c st (expr_app_2 (attributes_accessor_set acc) [v4; value_object ptr] nil) o ->
+    red_exprh k c st (expr_set_field_5 ptr obj (Some (attributes_accessor_of acc)) s v3 v4) o
+| red_exprh_set_field_5_unwritable : forall k c st ptr obj data s v3 v4,
+    attributes_data_writable data = false ->
+    red_exprh k c st (expr_set_field_5 ptr obj (Some (attributes_data_of data)) s v3 v4) (out_ter st (res_exception (value_string "unwritable-field")))
+| red_exprh_set_field_5_unextensible_add : forall k c st ptr obj s v3 v4,
+    object_extensible obj = false ->
+    red_exprh k c st (expr_set_field_5 ptr obj None s v3 v4) (out_ter st (res_value value_undefined))
+| red_exprh_set_field_5_unextensible_shadow : forall k c st ptr obj data s v3 v4,
+    attributes_data_writable data = true ->
+    get_object_property obj s = None ->
+    object_extensible obj = false ->
+    red_exprh k c st (expr_set_field_5 ptr obj (Some (attributes_data_of data)) s v3 v4) (out_ter st (res_value value_undefined))
+
+(* delete_field *)
+| red_exprh_delete_field : forall k c st e1 e2 o o',
+    red_exprh k c st e1 o ->
+    red_exprh k c st (expr_delete_field_1 o e2) o' ->
+    red_exprh (S k) c st (expr_delete_field e1 e2) o'
+| red_exprh_delete_field_1 : forall k c st' st v1 e2 o o',
+    red_exprh k c st e2 o ->
+    red_exprh k c st (expr_delete_field_2 v1 o) o' ->
+    red_exprh k c st' (expr_delete_field_1 (out_ter st (res_value v1)) e2) o'
+| red_exprh_delete_field_1_abort : forall k c st e2 o,
+    abort o ->
+    red_exprh k c st (expr_delete_field_1 o e2) o
+| red_exprh_delete_field_2 : forall k c st' st ptr s obj oattr o,
+    get_object st ptr = Some obj ->
+    get_object_property obj s = oattr ->
+    red_exprh k c st (expr_delete_field_3 ptr obj oattr s) o ->
+    red_exprh k c st' (expr_delete_field_2 (value_object ptr) (out_ter st (res_value (value_string s)))) o
+| red_exprh_delete_field_2_abort : forall k c st v1 o,
+    abort o ->
+    red_exprh k c st (expr_delete_field_2 v1 o) o
+| red_exprh_delete_field_3_not_found : forall k c st ptr obj s,
+    red_exprh k c st (expr_delete_field_3 ptr obj None s) (out_ter st (res_value value_false))
+| red_exprh_delete_field_3_unconfigurable : forall k c st ptr obj attr s,
+    attributes_configurable attr = false ->
+    red_exprh k c st (expr_delete_field_3 ptr obj (Some attr) s) (out_ter st (res_exception (value_string "unconfigurable-delete")))
+| red_exprh_delete_field_3_found : forall k c st st1 ptr obj attr s,
+    attributes_configurable attr = true ->
+    st1 = update_object st ptr (delete_object_property obj s) ->
+    red_exprh k c st (expr_delete_field_3 ptr obj (Some attr) s) (out_ter st1 (res_value value_true))
+
+(* own_field_names *)
+| red_exprh_own_field_names : forall k c st e o o',
+    red_exprh k c st e o ->
+    red_exprh k c st (expr_own_field_names_1 o) o' ->
+    red_exprh (S k) c st (expr_own_field_names e) o'
+| red_exprh_own_field_names_1 : forall k c st' st st1 ptr obj v,
+    get_object st ptr = Some obj ->
+    (st1, v) = add_object st (make_prop_list obj) ->
+    red_exprh k c st' (expr_own_field_names_1 (out_ter st (res_value (value_object ptr)))) (out_ter st1 (res_value v))
+| red_exprh_own_field_names_1_abort : forall k c st o,
+    abort o ->
+    red_exprh k c st (expr_own_field_names_1 o) o
+
+(* set_bang *)
+| red_exprh_set_bang : forall k c st i e o o',
+    red_exprh k c st e o ->
+    red_exprh k c st (expr_set_bang_1 i o) o' ->
+    red_exprh (S k) c st (expr_set_bang i e) o'
+| red_exprh_set_bang_1 : forall k c st' st st1 i loc v,
+    st1 = add_value_at_location st loc v ->
+    get_loc c i = Some loc -> 
+    red_exprh k c st' (expr_set_bang_1 i (out_ter st (res_value v))) (out_ter st1 (res_value v))
+| red_exprh_set_bang_1_abort : forall k c st i o,
+    abort o ->
+    red_exprh k c st (expr_set_bang_1 i o) o
+
+(* op1 *)
+| red_exprh_op1 : forall k c st e op o o',
+    red_exprh k c st e o ->
+    red_exprh k c st (expr_op1_1 op o) o' ->
+    red_exprh (S k) c st (expr_op1 op e) o'
+| red_exprh_op1_1 : forall k c st' st op v v',
+    unary_operator op st v = result_some v' ->
+    red_exprh k c st' (expr_op1_1 op (out_ter st (res_value v))) (out_ter st (res_value v'))
+| red_exprh_op1_1_abort : forall k c st op o,
+    abort o ->
+    red_exprh k c st (expr_op1_1 op o) o
+
+(* op2 *)
+| red_exprh_op2 : forall k c st e1 e2 op o o',
+    red_exprh k c st e1 o ->
+    red_exprh k c st (expr_op2_1 op o e2) o' ->
+    red_exprh (S k) c st (expr_op2 op e1 e2) o'
+| red_exprh_op2_1 : forall k c st' st e2 op v o o',
+    red_exprh k c st e2 o ->
+    red_exprh k c st (expr_op2_2 op v o) o' ->
+    red_exprh k c st' (expr_op2_1 op (out_ter st (res_value v)) e2) o'
+| red_exprh_op2_1_abort : forall k c st op e2 o,
+    abort o ->
+    red_exprh k c st (expr_op2_1 op o e2) o
+| red_exprh_op2_2 : forall k c st' st op v1 v2 v,
+    binary_operator op st v1 v2 = result_some v ->
+    red_exprh k c st' (expr_op2_2 op v1 (out_ter st (res_value v2))) (out_ter st (res_value v))
+| red_exprh_op2_2_abort : forall k c st op v o,
+    abort o ->
+    red_exprh k c st (expr_op2_2 op v o) o
+
+(* if *)
+| red_exprh_if : forall k c st e e1 e2 o o',
+    red_exprh k c st e o ->
+    red_exprh k c st (expr_if_1 o e1 e2) o' ->
+    red_exprh (S k) c st (expr_if e e1 e2) o'
+| red_exprh_if_1_true : forall k c st' st e1 e2 o,
+    red_exprh k c st e1 o ->
+    red_exprh k c st' (expr_if_1 (out_ter st (res_value value_true)) e1 e2) o
+| red_exprh_if_1_false : forall k c st' st e1 e2 o,
+    red_exprh k c st e2 o ->
+    red_exprh k c st' (expr_if_1 (out_ter st (res_value value_false)) e1 e2) o (* TODO: not-true-is-false? *)
+| red_exprh_if_1_abort : forall k c st e1 e2 o,
+    abort o ->
+    red_exprh k c st (expr_if_1 o e1 e2) o
+
+(* app *)
+| red_exprh_app : forall k c st e el o o',
+    red_exprh k c st e o ->
+    red_exprh k c st (expr_app_1 o el) o' ->
+    red_exprh (S k) c st (expr_app e el) o'
+| red_exprh_app_1 : forall k c st' st v el o,
+    red_exprh k c st (expr_app_2 v nil el) o ->
+    red_exprh k c st' (expr_app_1 (out_ter st (res_value v)) el) o
+| red_exprh_app_1_abort : forall k c st o el,
+    abort o ->
+    red_exprh k c st (expr_app_1 o el) o
+| red_exprh_app_2 : forall k c c' c'' st st' v ci is e vl vll o,
+    get_closure st v = result_some (value_closure ci c' is e) ->
+    (st', vll) = add_values st (rev vl) ->
+    add_parameters c' is vll = result_some c'' ->
+    red_exprh k c'' st' e o ->
+    red_exprh k c st (expr_app_2 v vl nil) o 
+| red_exprh_app_2_next : forall k c st v vl e el o o',
+    red_exprh k c st e o ->
+    red_exprh k c st (expr_app_3 v vl o el) o' ->
+    red_exprh k c st (expr_app_2 v vl (e :: el)) o'
+| red_exprh_app_3 : forall k c st' st v vl v' el o,
+    red_exprh k c st (expr_app_2 v (v' :: vl) el) o ->
+    red_exprh k c st' (expr_app_3 v vl (out_ter st (res_value v')) el) o
+| red_exprh_app_3_abort : forall k c st v vl el o,
+    abort o ->
+    red_exprh k c st (expr_app_3 v vl o el) o
+
+(* seq *)
+| red_exprh_seq : forall k c st e1 e2 o o',
+    red_exprh k c st e1 o ->
+    red_exprh k c st (expr_seq_1 o e2) o' ->
+    red_exprh (S k) c st (expr_seq e1 e2) o'
+| red_exprh_seq_1 : forall k c st' st v e2 o,
+    red_exprh k c st e2 o ->
+    red_exprh k c st' (expr_seq_1 (out_ter st (res_value v)) e2) o
+| red_exprh_seq_1_abort : forall k c st e2 o,
+    abort o ->
+    red_exprh k c st (expr_seq_1 o e2) o
+
+(* let *)
+| red_exprh_let : forall k c st i e1 e2 o o',
+    red_exprh k c st e1 o ->
+    red_exprh k c st (expr_let_1 i o e2) o' ->
+    red_exprh (S k) c st (expr_let i e1 e2) o'
+| red_exprh_let_1 : forall k c c1 st' st st1 i v e2 o,
+    (c1, st1) = add_named_value c st i v ->
+    red_exprh k c1 st1 e2 o ->
+    red_exprh k c st' (expr_let_1 i (out_ter st (res_value v)) e2) o
+| red_exprh_let_1_abort : forall k c st i o e2,
+    abort o ->
+    red_exprh k c st (expr_let_1 i o e2) o
+
+(* rec *)
+| red_exprh_rec : forall k c c1 st st1 loc i e1 e2 o o',
+    (c1, st1, loc) = add_named_value_loc c st i value_undefined ->
+    red_exprh k c1 st1 e1 o ->
+    red_exprh k c1 st1 (expr_recc_1 loc o e2) o' ->
+    red_exprh (S k) c st (expr_recc i e1 e2) o'
+| red_exprh_rec_1 : forall k c st' st st1 loc v e2 o,
+    st1 = add_value_at_location st loc v ->
+    red_exprh k c st1 e2 o ->
+    red_exprh k c st' (expr_recc_1 loc (out_ter st (res_value v)) e2) o
+| red_exprh_rec_1_abort : forall k c st loc o e2,
+    abort o ->
+    red_exprh k c st (expr_recc_1 loc o e2) o
+
+(* label *)
+| red_exprh_label : forall k c st i e o o',
+    red_exprh k c st e o ->
+    red_exprh k c st (expr_label_1 i o) o' ->
+    red_exprh (S k) c st (expr_label i e) o'
+| red_exprh_label_1 : forall k c st' i o,
+    (forall st v, o <> out_ter st (res_break i v)) ->
+    red_exprh k c st' (expr_label_1 i o) o
+| red_exprh_label_1_break : forall k c st' st i v,
+    red_exprh k c st' (expr_label_1 i (out_ter st (res_break i v))) (out_ter st (res_value v))
+
+(* break *)
+| red_exprh_break : forall k c st i e o o',
+    red_exprh k c st e o ->
+    red_exprh k c st (expr_break_1 i o) o' ->
+    red_exprh (S k) c st (expr_break i e) o'
+| red_exprh_break_1 : forall k c st' st i v,
+    red_exprh k c st' (expr_break_1 i (out_ter st (res_value v))) (out_ter st (res_break i v))
+| red_exprh_break_1_abort : forall k c st i o,
+    abort o ->
+    red_exprh k c st (expr_break_1 i o) o
+
+(* try_catch *)
+| red_exprh_try_catch : forall k c st e1 e2 o o',
+    red_exprh k c st e1 o ->
+    red_exprh k c st (expr_try_catch_1 o e2) o' ->
+    red_exprh (S k) c st (expr_try_catch e1 e2) o'
+| red_exprh_try_catch_1 : forall k c st e2 o,
+    (forall st v, o <> out_ter st (res_exception v)) -> (* TODO something better? *)
+    red_exprh k c st (expr_try_catch_1 o e2) o
+| red_exprh_try_catch_1_exc : forall k c st' st v e2 o o',
+    red_exprh k c st e2 o ->
+    red_exprh k c st (expr_try_catch_2 v o) o' ->
+    red_exprh k c st' (expr_try_catch_1 (out_ter st (res_exception v)) e2) o'
+| red_exprh_try_catch_2 : forall k c st' st v v' o,
+    red_exprh k c st (expr_app_2 v' [v] nil) o ->
+    red_exprh k c st' (expr_try_catch_2 v (out_ter st (res_value v'))) o
+| red_exprh_try_catch_2_abort : forall k c st v o,
+    abort o ->
+    red_exprh k c st (expr_try_catch_2 v o) o
+
+(* try_finally *)
+| red_exprh_try_finally : forall k c st e1 e2 o o',
+    red_exprh k c st e1 o ->
+    red_exprh k c st (expr_try_finally_1 o e2) o' ->
+    red_exprh (S k) c st (expr_try_finally e1 e2) o'
+| red_exprh_try_finally_1 : forall k c st' st r e2 o o',
+    red_exprh k c st e2 o ->
+    red_exprh k c st (expr_try_finally_2 r o) o' ->
+    red_exprh k c st' (expr_try_finally_1 (out_ter st r) e2) o'
+| red_exprh_try_finally_1_div : forall k c st e2,
+    red_exprh k c st (expr_try_finally_1 out_div e2) out_div
+| red_exprh_try_finally_2 : forall k c st' st r v,
+    red_exprh k c st' (expr_try_finally_2 r (out_ter st (res_value v))) (out_ter st r)
+| red_exprh_try_finally_2_abort : forall k c st r o,
+    abort o ->
+    red_exprh k c st (expr_try_finally_2 r o) o
+
+(* throw *)
+| red_exprh_throw : forall k c st e o o',
+    red_exprh k c st e o ->
+    red_exprh k c st (expr_throw_1 o) o' ->
+    red_exprh (S k) c st (expr_throw e) o'
+| red_exprh_throw_1 : forall k c st' st v,
+    red_exprh k c st' (expr_throw_1 (out_ter st (res_value v))) (out_ter st (res_exception v))
+| red_exprh_throw_1_abort : forall k c st o,
+    abort o ->
+    red_exprh k c st (expr_throw_1 o) o
+
+(* eval *)
+| red_exprh_eval : forall k c st e1 e2 o o',
+    red_exprh k c st e1 o ->
+    red_exprh k c st (expr_eval_1 o e2) o' ->
+    red_exprh (S k) c st (expr_eval e1 e2) o' 
+| red_exprh_eval_1 : forall k c st st' v1 e2 o o',
+    red_exprh k c st e2 o ->
+    red_exprh k c st (expr_eval_2 v1 o) o' -> 
+    red_exprh k c st' (expr_eval_1 (out_ter st (res_value v1)) e2) o'
+| red_exprh_eval_1_abort : forall k c st e2 o,
+    abort o ->
+    red_exprh k c st (expr_eval_1 o e2) o
+| red_exprh_eval_2 : forall k c c1 st' st st1 s e ptr obj o,
+    get_object st ptr = Some obj ->
+    envstore_of_obj st obj = Some (c1, st1) ->
+    desugar_expr s = Some e ->
+    red_exprh k c1 st1 e o ->
+    red_exprh k c st' (expr_eval_2 (value_string s) (out_ter st (res_value (value_object ptr)))) o
+| red_exprh_eval_2_abort : forall k c st v1 o,
+    abort o ->
+    red_exprh k c st (expr_eval_2 v1 o) o
+
+(* hint *)
+| red_exprh_hint : forall k c st s e o,
+    red_exprh k c st e o ->
+    red_exprh (S k) c st (expr_hint s e) o 
+.
+
