LambdaS5/coq/LjsPrettyRulesIndexedAux.v
@@ -1,0 +1,34 @@
+Generalizable All Variables.
+Set Implicit Arguments.
+Require Import LjsShared.
+Require Import LjsSyntax.
+Require Import LjsPrettyInterm.
+Require Import LjsPrettyRules.
+Require Import LjsPrettyRulesIndexed.
+Require Import LjsStore.
+Require Import LjsCommon.
+Require Import LjsValues.
+Require Import LjsOperators.
+Require Import LjsMonads.
+Require Import JsNumber.
+Require Import Coq.Strings.String.
+Import List.ListNotations.
+
+Open Scope list_scope.
+
+Implicit Type st : store.
+Implicit Type e : expr.
+Implicit Type v : value.
+Implicit Type loc : value_loc.
+Implicit Type s : string.
+Implicit Type n : number.
+Implicit Type i : id.
+Implicit Type o : out.
+Implicit Type c : ctx.
+Implicit Type ptr : object_ptr.
+Implicit Type obj : object.
+
+Lemma red_expr_add_h : forall c st e o, red_expr c st e o -> exists k, red_exprh k c st e o.
+Proof.
+(* TODO *)
+Admitted.
