LambdaS5/coq/make_indexed_rules.sed
@@ -1,0 +1,10 @@
+# change the name of the predicate
+s/red_expr/red_exprh/g
+# add the natural "depth" parameter
+s/Inductive red_exprh : /Inductive red_exprh : nat -> /g
+# add the parameter to quantifiers
+s/forall c/forall k c/g
+# add the parameter in the definition
+s/red_exprh c/red_exprh k c/g
+# increment the parameter, but only on the "big" steps
+s/red_exprh k c st (\(?expr_([a-z_]*|op[12])[ \)])/red_exprh (S k) c st \1/g
